\documentclass[12pt]{article}
\usepackage[utf8]{inputenc}
\usepackage{amsmath}
\usepackage{amssymb}
\usepackage{amsthm}

\begin{document}
Tenemos el resultado:
\begin{align}
  M^\nu_{11}= \frac{1}{16\pi^2}
  M_1 h_{11}h_{11}\left(c_R \,B_0(0,m_R^2,M_1^2)+
c_I \,B_0(0,m_I^2,M_1^2)  \right)
\end{align}
donde
\begin{align}
  B_0(r_{10}^2=0,m_R^2,M_1^2)=\frac{\left(2\pi\mu\right)^\epsilon}{i\pi^2}
\int d^dk\,\frac{1}{\left[(k+r_0)^2-m_R^2\right]}
\frac{1}{\left[(k+r_1)^2-m_R^2\right]}
\end{align}
Teniendo en cuenta que
\begin{align}
  r_{10}^2=&\left(r_1-r_0\right)^2=0
\end{align}
\begin{align}
  r_1-r_0=&0\nonumber\\
  r_1=&r_0
\end{align}
\begin{align}
  B_0(r_{10}^2=0,m_R^2,M_1^2)=\frac{\left(2\pi\mu\right)^\epsilon}{i\pi^2}
\int d^dk\,\frac{1}{\left[(k+r_0)^2-m_R^2\right]}
\frac{1}{\left[(k+r_0)^2-m_R^2\right]}
\end{align}

%\left(\right)
\end{document}
